Move all cheated map lemmas to mlmapTheory

basis/pure/mlmapScript.sml
@@ -8,7 +8,12 @@
 *)
 open preamble balanced_mapTheory
 
+val _ = set_grammar_ancestry ["balanced_map"];
+val _ = ParseExtras.tight_equality();
+
 val _ = new_theory"mlmap"
+
+(* implementation definitions *)
 
 val _ = Datatype `
   map = Map ('a -> 'a -> ordering) (('a, 'b) balanced_map)`;
@@ -48,5 +53,60 @@ val isSubmapBy_def = Define `
 
 val isSubmap_def = Define `
   isSubmap m1 m2 = isSubmapBy (=) m1 m2`;
+
+(* definitions for proofs *)
+
+val map_ok_def = Define `
+  map_ok (Map cmp t) <=> balanced_map$invariant cmp t /\ good_cmp cmp /\ TotOrd cmp`;
+
+val cmp_of_def = Define `
+  cmp_of (Map cmp t) = cmp`;
+
+(* theorems *)
+
+Theorem lookup_insert
+  `map_ok t ==>
+   lookup (insert t k1 v) k2 = if k1 = k2 then SOME v else lookup t k2`
+ (Cases_on `t`
+  \\ fs [map_ok_def,balanced_mapTheory.lookup_insert,lookup_def,insert_def]
+  \\ metis_tac [totoTheory.TotOrd])
+
+val to_fmap_def = Define `
+  to_fmap (Map cmp Tip) = FEMPTY /\
+  to_fmap (Map cmp (Bin s k v l r)) =
+    ((to_fmap (Map cmp l) ⊌ to_fmap (Map cmp r)) |+ (k,v))`;
+
+Theorem cmp_of_insert[simp]
+  `cmp_of (insert t k v) = cmp_of t`
+  (Cases_on `t` \\ fs [insert_def,cmp_of_def]);
+
+Theorem cmp_of_empty[simp]
+  `cmp_of (empty cmp) = cmp`
+  (fs [empty_def,cmp_of_def]);
+
+Theorem insert_thm
+  `map_ok t ==>
+   map_ok (insert t k v) /\
+   to_fmap (insert t k v) = (to_fmap t |+ (k, v))`
+  cheat;
+
+Theorem empty_thm
+  `(map_ok (empty cmp) = TotOrd cmp) /\ to_fmap (empty cmp) = FEMPTY`
+  (fs [empty_def,map_ok_def,balanced_mapTheory.empty_thm,
+      to_fmap_def,balanced_mapTheory.empty_def] \\ cheat)
+
+Theorem MAP_FST_toAscList
+  `map_ok t ⇒
+   SORTED (λx y. cmp_of t x y = Less) (MAP FST (toAscList t)) ∧
+   FDOM (to_fmap t) = set (MAP FST (toAscList t))`
+  cheat;
+
+Theorem MEM_toAscList
+  `map_ok t /\ MEM (k,v) (toAscList t) ==> FLOOKUP (to_fmap t) k = SOME v`
+  cheat;
+
+Theorem lookup_thm
+  `map_ok t ==> lookup t k = FLOOKUP (to_fmap t) k`
+  cheat;
 
 val _ = export_theory()
